WIP proposal for Hash that hashes the word in register, instead of capability ; capability are hashed by software

theories/rules/rules_Hash.v
@@ -20,639 +20,218 @@ Section cap_lang_rules.
   Implicit Types mem : Mem.
   Implicit Types lmem : LMem.
 
-  Definition reg_allows_hash (lregs : LReg) (r : RegName) p b e a v :=
-    lregs !! r = Some (LCap p b e a v) ∧ readAllowed p = true.
-
-  (* Definition hash_lmemory_region (lm : LMem) (b e : Addr) (v : Version) := *)
-  (*   let instructions : list LWord := *)
-  (*     map snd *)
-  (*       ((map_to_list *)
-  (*           (filter (fun mem_addr => (laddr_get_addr (fst mem_addr)) ∈ (finz.seq_between b e) *)
-  (*                                 /\ (laddr_get_version (fst mem_addr)) = v) *)
-  (*              lm))) *)
-  (*   in *)
-  (*   hash (fmap lword_get_word instructions). *)
-
-  Inductive Hash_failure (lregs: LReg) (dst src: RegName) (lmem : LMem) :=
-  | Hash_fail_const lw:
-      lregs !! src = Some lw ->
-      is_log_cap lw = false →
-      Hash_failure lregs dst src lmem
-  | Hash_fail_perm p b e a v:
-      lregs !! src = Some (LCap p b e a v) ->
-      readAllowed p = false →
-      Hash_failure lregs dst src lmem
-  (* Notice how the None below also includes all cases where we read an inl value into the PC, because then incrementing it will fail *)
-  | Hash_fail_invalid_PC p b e a v :
-      lregs !! src = Some (LCap p b e a v) ->
-      Forall (fun a => ∃ lw, lmem !! (a,v) = Some lw) (finz.seq_between b e) ->
-      incrementLPC (<[ dst := LInt (hash_lmemory_region lmem b e v)]> lregs) = None ->
-      Hash_failure lregs dst src lmem
-  .
-
-  Inductive Hash_spec (lregs: LReg) (dst src: RegName) (lmem : LMem) (lregs': LReg): cap_lang.val -> Prop :=
-  | Hash_spec_success p b e a v :
-      reg_allows_hash lregs src p b e a v ->
-      Forall (fun a => ∃ w, lmem !! (a,v) = Some w) (finz.seq_between b e) ->
-      incrementLPC (<[ dst := LInt (hash_lmemory_region lmem b e v)]> lregs) = Some lregs' ->
-      Hash_spec lregs dst src lmem lregs' NextIV
-  | Hash_spec_failure:
-    lregs = lregs' ->
-    Hash_failure lregs dst src lmem ->
-    Hash_spec lregs dst src lmem lregs' FailedV.
-
-  Definition allow_hash_map_or_true r (lregs : LReg) (lmem : LMem):=
-    ∃ p b e a v, read_reg_inr lregs r p b e a v ∧
-      if decide (reg_allows_hash lregs r p b e a v)
-      then Forall (fun a => ∃ lw, lmem !! (a,v) = Some lw) (finz.seq_between b e)
-      else True.
-
-  Lemma allow_hash_implies_hashv:
-    ∀ (src : RegName) (lmem : LMem) (lr : LReg) (p : Perm) (b e a : Addr) v,
-      allow_hash_map_or_true src lr lmem
-      → lr !! src = Some (LCap p b e a v)
-      → readAllowed p = true
-      → Forall (fun a => ∃ lw, lmem !! (a,v) = Some lw) (finz.seq_between b e).
-  Proof.
-    intros src lmem lr p b e a v HaHash Hr2v Hra.
-    unfold allow_hash_map_or_true, read_reg_inr in HaHash.
-    destruct HaHash as (?&?&?&?&?& Hrinr & Hmem).
-    rewrite Hr2v in Hrinr. inversion Hrinr; subst.
-    case_decide as Hrega.
-    - exact Hmem.
-    - contradiction Hrega. done.
-  Qed.
-
-  Lemma incrementLPC_incrementPC_some regs regs' :
-    incrementLPC regs = Some regs' ->
-    incrementPC (lreg_strip regs) = Some (lreg_strip regs').
-  Proof.
-    rewrite /incrementPC /incrementLPC.
-    intros Hlpc.
-    rewrite /lreg_strip lookup_fmap; cbn.
-    destruct (regs !! PC) as [lw|] eqn:Heq ; rewrite Heq; cbn in *; last done.
-    destruct_lword lw; cbn in *; try done.
-    destruct (a + 1)%a; last done.
-    simplify_eq.
-    by rewrite fmap_insert.
-  Qed.
-
-  Lemma incrementLPC_incrementPC_none regs :
-    incrementLPC regs = None <-> incrementPC (lreg_strip regs) = None.
-  Proof.
-    intros.
-    rewrite /incrementPC /incrementLPC.
-    rewrite /lreg_strip lookup_fmap; cbn.
-    destruct (regs !! PC) as [LX|] eqn:Heq ; rewrite Heq; cbn; last done.
-    destruct LX ; cbn ; [(clear; firstorder) | | (clear; firstorder)].
-    destruct sb as [? ? ? a' | ] ; eauto; cbn; last done.
-    destruct (a' + 1)%a eqn:Heq'; done.
-  Qed.
-
-  Lemma incrementLPC_fail_updatePC regs m etbl ecur:
-    incrementLPC regs = None ->
-    updatePC {| reg := (lreg_strip regs); mem := m; etable := etbl ; enumcur := ecur |} = None.
-  Proof.
-    intro Hincr. apply incrementLPC_incrementPC_none in Hincr.
-    by apply incrementPC_fail_updatePC.
-  Qed.
-
-
-  Lemma incrementLPC_success_updatePC regs m etbl ecur regs' :
-    incrementLPC regs = Some regs' ->
-    ∃ p b e a a' (v : Version),
-      regs !! PC = Some (LCap p b e a v) ∧
-      (a + 1)%a = Some a' ∧
-      updatePC {| reg := (lreg_strip regs); mem := m; etable := etbl ; enumcur := ecur |} =
-      Some (NextI,
-              {| reg := (<[PC:=WCap p b e a']> (lreg_strip regs));
-                mem := m;
-                etable := etbl ;
-                enumcur := ecur |})
-      ∧ regs' = <[ PC := (LCap p b e a' v) ]> regs.
-  Proof.
-    intro Hincr.
-    opose proof (incrementLPC_incrementPC_some _ _ Hincr) as HincrPC.
-    eapply (incrementPC_success_updatePC _ m etbl ecur) in HincrPC.
-    destruct HincrPC as (p'&b'&e'&a''&a'''&Hregs&Heq&Hupd&Hregseq).
-    rewrite /incrementLPC in Hincr.
-    destruct (regs !! PC) as [wpc |]; last done.
-    destruct_lword wpc; try done.
-    destruct (a + 1)%a as [a'|] eqn:Heq'; last done; simplify_eq.
-    rewrite /lreg_strip fmap_insert //= -/(lreg_strip regs)  in Hregseq.
-    exists p, b, e, a, a', v.
-    repeat (split; try done).
-    by rewrite Hupd Hregseq.
-  Qed.
+  Inductive Hash_spec (lregs: LReg) (dst src: RegName) (lregs': LReg): cap_lang.val -> Prop :=
+  | Hash_spec_success lwsrc :
+    lregs !! src = Some lwsrc ->
+    incrementLPC (<[ dst := LWInt (hash (lword_get_word lwsrc))]> lregs) = Some lregs' ->
+    Hash_spec lregs dst src lregs' NextIV
+  | Hash_spec_failure lwsrc:
+    incrementLPC (<[ dst := LWInt (hash (lword_get_word lwsrc))]> lregs) = None →
+    Hash_spec lregs dst src lregs' FailedV.
 
   Definition exec_optL_Hash
-    (lregs : LReg) (lmem : LMem)
-    (dst src : RegName) : option LReg :=
-    lwsrc ← lregs !! src ;
-    match lwsrc with
-    | LCap p b e a v =>
-        if readAllowed p
-        then
-          lpc ← incrementLPC (<[dst := (LWInt (hash_lmemory_region lmem b e v)) ]> lregs) ;
-          Some lpc (* trick to bind with update_reg *)
-        else None
-    | _ => None
-    end.
+    (lregs : LReg) (dst src : RegName) : option LReg :=
+    lwsrc ← lregs !! src;
+    lpc ← incrementLPC (<[dst := LWInt (hash (lword_get_word lwsrc)) ]> lregs) ;
+    Some lpc.
 
-  Lemma hash_lmemory_weaken lmem lm b e v :
-    Forall (λ a : Addr, ∃ lw, lmem !! (a, v) = Some lw) (finz.seq_between b e) ->
-    lmem ⊆ lm ->
-    (hash_lmemory_region lm b e v) =
-    (hash_lmemory_region lmem b e v).
-  Proof.
-    revert lm.
-    rewrite /hash_lmemory_region.
-    induction lmem using map_ind; intros lm Hall Hmem.
-    - f_equal.
-      match goal with | _ : _ |- context [ (filter ?f lm) ] => set (Flm := f) end.
-      pose proof (map_filter_empty_iff Flm lm) as [_ HFlm].
-      rewrite HFlm.
-      + by rewrite map_filter_empty map_to_list_empty !fmap_nil.
-      + subst Flm.
-        apply map_Forall_lookup_2.
-        intros [a v'] lw Hlw; cbn.
-        intro Hcontra.
-        destruct Hcontra as [Hcontra ->].
-        rewrite Forall_forall in Hall.
-        apply Hall in Hcontra.
-        set_solver.
-    - f_equal.
-      match goal with | _ : _ |- context [ (filter ?f lm) ] => set (Flm := f) end.
-      assert (lm = (<[i := x]> lm)) as Hlm_eq.
-      { rewrite insert_id; first done.
-        by eapply insert_weaken.
-      }
-      rewrite Hlm_eq.
-      apply insert_subseteq_r_inv in Hmem ; auto.
-      rewrite !map_filter_insert.
-      destruct (decide (Flm (i, x))).
-      + admit.
-      + rewrite !map_filter_delete.
-  Admitted.
+  (* Lemma hash_lmemory_weaken lmem lm b e v : *)
+  (*   Forall (λ a : Addr, ∃ lw, lmem !! (a, v) = Some lw) (finz.seq_between b e) -> *)
+  (*   lmem ⊆ lm -> *)
+  (*   (hash_lmemory_region lm b e v) = *)
+  (*   (hash_lmemory_region lmem b e v). *)
+  (* Proof. *)
+  (*   revert lm. *)
+  (*   rewrite /hash_lmemory_region. *)
+  (*   induction lmem using map_ind; intros lm Hall Hmem. *)
+  (*   - f_equal. *)
+  (*     match goal with | _ : _ |- context [ (filter ?f lm) ] => set (Flm := f) end. *)
+  (*     pose proof (map_filter_empty_iff Flm lm) as [_ HFlm]. *)
+  (*     rewrite HFlm. *)
+  (*     + by rewrite map_filter_empty map_to_list_empty !fmap_nil. *)
+  (*     + subst Flm. *)
+  (*       apply map_Forall_lookup_2. *)
+  (*       intros [a v'] lw Hlw; cbn. *)
+  (*       intro Hcontra. *)
+  (*       destruct Hcontra as [Hcontra ->]. *)
+  (*       rewrite Forall_forall in Hall. *)
+  (*       apply Hall in Hcontra. *)
+  (*       set_solver. *)
+  (*   - f_equal. *)
+  (*     match goal with | _ : _ |- context [ (filter ?f lm) ] => set (Flm := f) end. *)
+  (*     assert (lm = (<[i := x]> lm)) as Hlm_eq. *)
+  (*     { rewrite insert_id; first done. *)
+  (*       by eapply insert_weaken. *)
+  (*     } *)
+  (*     rewrite Hlm_eq. *)
+  (*     apply insert_subseteq_r_inv in Hmem ; auto. *)
+  (*     rewrite !map_filter_insert. *)
+  (*     destruct (decide (Flm (i, x))). *)
+  (*     + admit. *)
+  (*     + rewrite !map_filter_delete. *)
+  (* Admitted. *)
 
   Lemma wp_hash Ep
     pc_p pc_b pc_e pc_a pc_v
-    dst src lw lmem lregs :
+    dst src lw lregs :
     decodeInstrWL lw = Hash dst src →
     isCorrectLPC (LCap pc_p pc_b pc_e pc_a pc_v) →
     lregs !! PC = Some (LCap pc_p pc_b pc_e pc_a pc_v) →
     regs_of (Hash dst src) ⊆ dom lregs →
-    lmem !! (pc_a, pc_v) = Some lw →
-    allow_hash_map_or_true src lregs lmem →
 
-    {{{ (▷ [∗ map] la↦lw ∈ lmem, la ↦ₐ lw) ∗
-          ▷ [∗ map] k↦y ∈ lregs, k ↦ᵣ y }}}
+    {{{ ▷ (pc_a, pc_v) ↦ₐ lw ∗
+        ▷ [∗ map] k↦y ∈ lregs, k ↦ᵣ y }}}
       Instr Executable @ Ep
       {{{ lregs' retv, RET retv;
-          ⌜ Hash_spec lregs dst src lmem lregs' retv⌝ ∗
-            ([∗ map] la↦lw ∈ lmem, la ↦ₐ lw) ∗
-            [∗ map] k↦y ∈ lregs', k ↦ᵣ y }}}.
+          ⌜ Hash_spec lregs dst src lregs' retv⌝ ∗
+          (pc_a, pc_v) ↦ₐ lw ∗
+          [∗ map] k↦y ∈ lregs', k ↦ᵣ y }}}.
   Proof.
-    iIntros (Hinstr Hvpc HPC Dregs Hmem_pc HaHash φ) "(>Hmem & >Hmap) Hφ".
-    apply isCorrectLPC_isCorrectPC_iff in Hvpc; cbn in Hvpc.
-    iApply wp_lift_atomic_head_step_no_fork; auto.
-    iIntros (σ1 ns l1 l2 nt) "Hσ1 /=". destruct σ1; simpl.
-    iDestruct "Hσ1" as (lr lm vmap tbl_cur tbl_prev tbl_all)
-        "(Hr & Hm
-         & -> & Htbl_cur & Htbl_prev & Htbl_all
-         & HEC
-         & %Hdom_tbl1 & %Hdom_tbl2 & %Hdom_tbl3 & %Hdom_tbl4
-         & %HLinv)"
-    ; cbn in HLinv, Hdom_tbl1, Hdom_tbl2, Hdom_tbl3, Hdom_tbl4.
-    pose proof HLinv as HLinv'.
+    iIntros (Hinstr Hvpc HPC Dregs φ) "(>Hpc_a & >Hmap) Hφ".
 
-    (* Derive necessary register values in r *)
-    iDestruct (gen_heap_valid_inclSepM with "Hr Hmap") as %Hregs.
-    have Hregs_pc := lookup_weaken _ _ _ _ HPC Hregs.
-    specialize (indom_lregs_incl _ _ _ Dregs Hregs) as Hri. unfold regs_of in Hri.
-    odestruct (Hri dst) as [ldstv [Hldst' Hldst] ]; first by set_solver+.
-    odestruct (Hri src) as [lsrcv [Hlsrc' Hlsrc] ]; first by set_solver+.
-
-    (* Derive necessary memory *)
-    iDestruct (gen_heap_valid_inclSepM with "Hm Hmem") as %Hmem.
-    iDestruct (gen_mem_valid_inSepM lmem lm with "Hm Hmem") as %Hma; eauto.
-
+    iApply (wp_instr_exec_opt Hvpc HPC Hinstr Dregs with "[$Hpc_a $Hmap Hφ]").
     iModIntro.
-    iSplitR.
-    by iPureIntro; apply normal_always_head_reducible.
-    iNext. iIntros (e2 σ2 efs Hpstep).
-    apply prim_step_exec_inv in Hpstep as (-> & -> & (c & -> & Hstep)).
-    iIntros "_".
-    iSplitR; auto; eapply step_exec_inv in Hstep; eauto.
-    2: rewrite -/((lword_get_word (LCap pc_p pc_b pc_e pc_a pc_v)))
-    ; eapply state_corresponds_reg_get_word ; eauto.
-    2: eapply state_corresponds_mem_correct_PC ; eauto; cbn ; eauto.
+    iIntros (σ) "(Hσ & Hregs &Hpc_a)".
+    iModIntro.
+    iIntros (wa) "(%Hppc & %Hpmema & %Hcorrpc & %Hdinstr) Hcred".
 
-    set (srcv := lword_get_word lsrcv).
-    assert ( reg !! src = Some srcv ) as Hsrc
-        by (eapply state_corresponds_reg_get_word ; eauto).
-    rewrite /exec /= Hsrc /= in Hstep.
+    iApply (wp_wp2 (φ1 := exec_optL_Hash lregs dst src)).
+    iApply wp_opt2_bind.
+    iApply wp_opt2_eqn.
+    iMod (state_interp_transient_intro (lm:= ∅) with "[$Hregs $Hσ]") as "Hσ". set_solver.
+    iApply (wp2_reg_lookup (lrt := lregs)); first by set_solver.
+    iModIntro.
+    iFrame "Hσ".
+    iIntros (lwr) "Hσ %Hlrs %Hrs".
 
+    iDestruct (update_state_interp_transient_from_regs_mod (dst := dst) (lw2 := LInt (hash (lword_get_word lwr))) with "Hσ") as "Hσ".
+    { now set_solver. }
+    { now intros. }
 
-    (* src contains a capability *)
-    destruct (is_log_cap lsrcv) eqn:Hlsrcv; cycle 1; subst srcv; cbn in *.
-    { (* Fail : not a capability *)
-      destruct_lword lsrcv; cbn in * ; try congruence; clear Hlsrcv.
-      all: simplify_map_eq.
-      all: (iSplitR "Hφ Hmap Hmem"
-            ; [ iExists lr, lm, vmap,_,_,_; iFrame; auto
-              | iApply "Hφ" ; iFrame ; iFailCore Hash_fail_const
+    rewrite updatePC_incrementPC.
+    iApply (wp_opt2_bind (φ1 := incrementLPC (<[ dst := LInt (hash (lword_get_word lwr))]> lregs)) (k1 := (fun x => Some x))).
+    iApply wp_opt2_eqn_both.
 
-           ]).
-    }
-    destruct_lword lsrcv ; try (cbn in * ; congruence).
-    cbn in Hstep.
-
-
-    destruct (readAllowed p) eqn:HaRead; cycle 1; cbn in *.
-    {
-      simplify_map_eq.
-      iSplitR "Hφ Hmap Hmem"
-            ; [ iExists lr, lm, vmap,_,_,_; iFrame; auto
-              | iApply "Hφ" ; iFrame ; iFailCore Hash_fail_perm
-        ].
-    }
-
-    set (lregs' := (<[ dst := LInt (hash_lmemory_region lm b e v) ]> lregs)).
-    set (lr' := (<[ dst := LInt (hash_lmemory_region lm b e v) ]> lr)).
-    assert (lreg_strip lregs' ⊆ lreg_strip lr') as Hlregs'_in_lr'.
-    { subst lregs' lr'.
-      by apply map_fmap_mono, insert_mono.
-    }
-
-
-    assert ( (lreg_strip lr') =
-               (<[ dst := WInt (hash_memory_region mem b e) ]> reg))
-      as Hstrip_lr'.
-    { subst lr'.
-      destruct HLinv as [ [Hstrips Hcurreg] _].
-      rewrite -Hstrips /lreg_strip !fmap_insert -/(lreg_strip lr) //=.
-      erewrite lmeasure_measure; eauto.
-    }
-
-    destruct (incrementLPC lregs') as  [?|] eqn:Hlregs'
-    ; pose proof Hlregs' as H'lregs'
-    ; cycle 1.
-    {
-      apply incrementLPC_fail_updatePC with (m:=mem) (etbl:=etable) (ecur:=enumcur) in Hlregs'.
-      eapply updatePC_fail_incl with
-        (regs' := lreg_strip lr') (m':=mem)
-        (etbl':=etable) (ecur':=enumcur) in Hlregs'
-      ; auto
-      ; cycle 1.
-      {
-        rewrite /lreg_strip lookup_fmap.
-        subst lregs' lr'.
-        apply fmap_is_Some.
-        destruct (decide (dst = PC)); simplify_map_eq ; auto.
-      }
-      rewrite Hstrip_lr' in Hlregs'.
-      match goal with
-      | Hstep :
-        match ?x with _ => _ end = (_,_) |- _ =>
-          replace x with (None : option Conf) in Hstep
-            by (destruct_lword lsrcv ; eauto)
-      end
-      ; simplify_eq.
-      subst lr'.
-
-      iSplitR "Hφ Hmap Hmem"
-      ; [ iExists lr, lm, vmap,_,_,_; iFrame; auto
-        | iApply "Hφ" ; iFrame].
-      eapply allow_hash_implies_hashv in HaHash; eauto.
-      subst lregs'.
-      rewrite {1}(hash_lmemory_weaken lmem lm) in H'lregs'; eauto.
-      cbn in *; iFailCore Hash_fail_invalid_PC.
-    }
-
-    (* PC has been incremented correctly *)
-    rewrite /update_reg /= in Hstep.
-    eapply (incrementLPC_success_updatePC _ mem etable enumcur) in Hlregs'
-        as (p1 & b1 & e1 & a1 & a_pc1 & v1 & HPC'' & Ha_pc' & HuPC & ->)
-    ; simplify_map_eq.
-    assert (dst <> PC) as Hdst by (subst lregs' ; intro ; simplify_map_eq).
-    eapply updatePC_success_incl with
-      (regs' := lreg_strip lr') (m':=mem) (etbl':=etable) (ecur':=enumcur) in HuPC
-    ; auto.
-    rewrite Hstrip_lr' in HuPC.
-    rewrite HuPC in Hstep; clear HuPC.
-    subst lregs' lr' ; simplify_eq ; simplify_map_eq.
-    eapply allow_hash_implies_hashv in HaHash; eauto.
-
-
-    iMod ((gen_heap_update_inSepM _ _ dst (LInt (hash_lmemory_region lm b e v))) with "Hr Hmap")
-      as "[Hr Hmap]"; eauto.
-    iMod ((gen_heap_update_inSepM _ _ PC (LCap p1 b1 e1 a_pc1 v1)) with "Hr Hmap")
-      as "[Hr Hmap]"; eauto ; first by simplify_map_eq.
-
-    rewrite {1}(hash_lmemory_weaken lmem lm) in H'lregs'; eauto.
-
-
-    iFrame; iModIntro ; iSplitR "Hφ Hmap Hmem"
-    ; [| iApply "Hφ" ; iFrame; iPureIntro ; eapply Hash_spec_success; eauto]; cycle 1.
-    { split; eauto. }
-
-    iExists _, lm, vmap,_,_,_; iFrame; auto
-    ; iPureIntro; econstructor; eauto
-    ; repeat (split ; first done)
-    ; destruct HLinv as [ [Hstrips Hcur_reg] [Hdom Hroot] ]
-    ; cbn in *
-    ; last (split;eauto)
-    ; last done.
-    assert ( is_cur_word (LCap p1 b1 e1 a_pc1 v1) vmap ) as Hcur_PC.
-    { eapply lookup_weaken in HPC'' ; eauto.
-      eapply is_cur_lword_lea with (a' := a_pc1) ; cycle 2 ; eauto ; apply isWithin_refl.
-    }
-    erewrite lmeasure_measure; eauto.
-    eapply lreg_corresponds_insert_respects; eauto.
-    eapply lreg_corresponds_insert_respects; done.
+    iApply (wp2_opt_incrementPC with "[$Hσ Hpc_a Hφ]").
+    { rewrite dom_insert. apply elem_of_union_r. now rewrite elem_of_dom HPC. }
+    iSplit.
+    - iIntros (φt' lrt') "Hσ %Hlin %Hin".
+      iDestruct (state_interp_transient_elim_abort with "Hσ") as "(Hσ & Hregs & _)".
+      iFrame.
+      iApply ("Hφ" with "[$Hpc_a $Hregs]").
+      iPureIntro.
+      by eapply Hash_spec_failure.
+    - iIntros (regs' φt') "Hσ %Hlis %His".
+      iApply wp2_val.
+      cbn.
+      iMod (state_interp_transient_elim_commit with "Hσ") as "($ & Hregs & _)".
+      iApply ("Hφ" with "[$Hpc_a $Hregs]").
+      iPureIntro.
+      eapply Hash_spec_success; try eassumption.
   Qed.
-
-  (* TODO old proof *)
-  (*   iIntros (Hinstr Hvpc HPC Dregs Hmem_pc HaHash φ) "(>Hmem & >Hregs) Hφ". *)
-  (*   rewrite -(insert_id lmem _ _ Hmem_pc). *)
-  (*   iDestruct (big_sepM_insert_delete with "Hmem") as "[Hpc_a Hmem]"; cbn. *)
-
-  (*   iApply (wp_instr_exec_opt Hvpc HPC Hinstr Dregs with "[$Hpc_a $Hregs Hmem Hφ]"). *)
-
-  (*   iModIntro. *)
-  (*   iIntros (σ) "(Hσ & Hregs &Hpc_a)". *)
-  (*   iModIntro. *)
-  (*   iIntros (wa) "(%Hppc & %Hpmema & %Hcorrpc & %Hdinstr) Hcred". *)
-
-  (*   iApply (wp_wp2 (φ1 := exec_optL_Hash lregs lmem dst src)). *)
-  (*   iApply wp_opt2_bind. *)
-  (*   iApply wp_opt2_eqn. *)
-
-  (*   iDestruct (big_sepM_insert_delete _ _ _ lw with "[Hpc_a $Hmem]") as "Hmem"; iFrame. *)
-  (*   rewrite insert_id; auto. *)
-  (*   iMod (state_interp_transient_intro_nodfracs with "[$Hregs $Hσ $Hmem]") as "Hσ". *)
-
-  (*   iApply (wp2_reg_lookup with "[$Hσ Hφ Hcred]") ; first by set_solver. *)
-  (*   iIntros (lw2) "Hσ %Hlrs %Hrs". *)
-
-  (*   destruct (is_log_cap lw2) eqn:Hlw2; cycle 1. *)
-  (*   { *)
-  (*     destruct_lword lw2 ; cbn in * ; simplify_eq. *)
-  (*     all: iModIntro. *)
-  (*     all: iDestruct (state_interp_transient_elim_abort with "Hσ") as "($ & Hregs & Hmem)". *)
-  (*     all: rewrite big_sepM_fmap. *)
-  (*     all: iApply ("Hφ" with "[$Hmem $Hregs]"). *)
-  (*     all: iPureIntro; constructor; by eapply Hash_fail_const. *)
-  (*   } *)
-
-  (*   destruct_lword lw2 ; cbn in * ; simplify_eq. *)
-  (*   destruct (decide (readAllowed p = true)) as [Hread|Hread] *)
-  (*   ; [|apply not_true_is_false in Hread] ; rewrite Hread ;cycle 1;cbn. *)
-  (*   { *)
-  (*     iModIntro. *)
-  (*     iDestruct (state_interp_transient_elim_abort with "Hσ") as "($ & Hregs & Hmem)". *)
-  (*     rewrite big_sepM_fmap. *)
-  (*     iApply ("Hφ" with "[$Hmem $Hregs]"). *)
-  (*     iPureIntro; constructor; by eapply Hash_fail_perm. *)
-  (*   } *)
-
-  (*   pose proof (allow_hash_implies_hashv _ _ _ _ _ _ _ _ HaHash Hlrs Hread) as Hhash_mem. *)
-
-  (*   rewrite updatePC_incrementPC. *)
-  (*   iApply (wp_opt2_bind (k1 := fun x => Some x)). *)
-  (*   iApply wp_opt2_eqn_both. *)
-
-  (*   iDestruct (update_state_interp_transient_from_regs_mod (dst := dst) (lw2 := LInt (hash_lmemory_region lmem b e v)) with "Hσ") as "Hσ". *)
-  (*   { set_solver. } *)
-  (*   { by cbn. } *)
-
-  (*   replace (WInt (hash_memory_region (mem σ) b e)) *)
-  (*     with ( lword_get_word  (LInt (hash_lmemory_region lmem b e v))). *)
-  (*   2:{ cbn. admit. } *)
-
-
-  (*   iApply (wp2_opt_incrementPC with "[$Hσ Hcred Hφ]"). *)
-  (*   { now rewrite elem_of_dom (lookup_insert_dec HPC). } *)
-  (*   iSplit; cbn; iIntros (φt' lrt') "Hσ %Heqn1 %Heqn2". *)
-  (*   - iDestruct (state_interp_transient_elim_abort with "Hσ") as "($ & Hregs & Hmem)". *)
-  (*     rewrite big_sepM_fmap. *)
-  (*     iApply ("Hφ" with "[$Hmem $Hregs]"). *)
-  (*     iPureIntro. *)
-  (*     eapply Hash_spec_failure. *)
-  (*     by econstructor. *)
-  (*   - iApply wp2_val. *)
-  (*     cbn. *)
-  (*     iMod (state_interp_transient_elim_commit with "Hσ") as "($ & Hregs & Hmem)". *)
-  (*     rewrite big_sepM_fmap. *)
-  (*     iApply ("Hφ" with "[$Hmem $Hregs]"). *)
-  (*     iPureIntro. *)
-  (*     eapply Hash_spec_success; eauto. *)
-  (*     split;eauto. *)
-  (* Admitted. *)
-
-(* Global Instance laddr_eqdec: EqDecision LAddr. *)
-(* Proof. apply _. Defined. *)
-(* Global Instance laddr_countable: Countable LAddr. *)
-(* Admitted. *)
-
 
   Lemma wp_hash_success Ep
     pc_p pc_b pc_e pc_a pc_a' pc_v
     dst src
-    wdst p b e a v ws lw
+    wdst wsrc lw
     :
 
     decodeInstrWL lw = Hash dst src →
     isCorrectLPC (LCap pc_p pc_b pc_e pc_a pc_v) →
-    readAllowed p = true →
     (pc_a + 1)%a = Some pc_a' →
-    pc_a ∉ finz.seq_between b e ->
-    length ws = finz.dist b e ->
 
     {{{ ▷ PC ↦ᵣ LCap pc_p pc_b pc_e pc_a pc_v
         ∗ ▷ (pc_a, pc_v) ↦ₐ lw
         ∗ ▷ dst ↦ᵣ wdst
-        ∗ ▷ src ↦ᵣ LCap p b e a v
-        ∗ ▷ [[ b , e ]] ↦ₐ{ v } [[ ws ]]
+        ∗ ▷ src ↦ᵣ wsrc
     }}}
       Instr Executable @ Ep
       {{{ RET NextIV;
           PC ↦ᵣ LCap pc_p pc_b pc_e pc_a' pc_v
           ∗ (pc_a, pc_v) ↦ₐ lw
-          ∗ dst ↦ᵣ LWInt (hash (lword_get_word <$> ws))
-          ∗ src ↦ᵣ LCap p b e a v
-          ∗ [[ b , e ]] ↦ₐ{ v } [[ ws ]]
+          ∗ dst ↦ᵣ LWInt (hash (lword_get_word wsrc))
+          ∗ src ↦ᵣ wsrc
       }}}.
   Proof.
-    intros Hdecode HcorrectPC Hread_allowed Hpca' Hpca_ne Hlen_ws.
-    iIntros (φ) "(>HPC & >Hpca & >Hdst & >Hsrc & >Hmem) Hφ".
+    intros Hdecode HcorrectPC Hpca'.
+    iIntros (φ) "(>HPC & >Hpca & >Hdst & >Hsrc) Hφ".
     iDestruct (map_of_regs_3 with "HPC Hdst Hsrc") as "[Hmap (%&%&%)]".
     rewrite /region_mapsto.
-    iDestruct ( big_sepL2_to_big_sepM with "Hmem") as "Hmem".
-    { apply NoDup_fmap_2.
-      - intros a1 a2 Haeq; congruence.
-      - by apply finz_seq_between_NoDup.
-    }
-    iDestruct (big_sepM_insert with "[$Hmem $Hpca]") as "Hmem".
-    { shelve. }
-
     iApply (wp_hash with "[$]"); eauto.
     { by simplify_map_eq. }
     { by rewrite !dom_insert; set_solver+. }
-    { by simplify_map_eq. }
-    {
-      rewrite /allow_hash_map_or_true.
-      exists p,b,e,a,v.
-      split.
-      - rewrite /read_reg_inr.
-        rewrite lookup_insert_ne //.
-        rewrite lookup_insert_ne //.
-        by simplify_map_eq.
-      - match goal with
-        | H: _ |- context [decide ?x] => destruct (decide x)
-        end; last done.
-        apply Forall_forall.
-        intros a' Ha'.
-        destruct (decide (a' = pc_a)); simplify_map_eq.
-        rewrite lookup_insert_ne; last congruence.
-        rewrite -/(is_Some (_ !! (a',v))).
-        apply elem_of_dom.
-        rewrite dom_list_to_map_L.
-        apply elem_of_list_to_set.
-        rewrite fst_zip.
-        2: { by rewrite Hlen_ws map_length finz_seq_between_length. }
-        apply elem_of_list_fmap.
-        eexists ; split; done.
-    }
-    iNext. iIntros (lregs' retv) "(%Hspec & Hmem & Hregs)".
+    iNext. iIntros (lregs' retv) "(%Hspec & Hpca & Hregs)".
     destruct Hspec; cycle 1.
-    { destruct X; simplify_map_eq; try congruence.
-      incrementLPC_inv; simplify_map_eq; eauto; congruence.
-    }
+    { incrementLPC_inv; simplify_map_eq; eauto; congruence. }
     iApply "Hφ".
     incrementLPC_inv; simplify_map_eq; eauto.
     rewrite (insert_commute _ PC dst) // insert_insert.
     rewrite (insert_commute _ dst PC) // insert_insert.
     iDestruct (regs_of_map_3 with "Hregs") as "(?&?&?)"; eauto; iFrame.
+  Qed.
 
-    replace
-      (hash_lmemory_region (<[(x2, x3):=lw]> (list_to_map (zip (map (λ a1 : Addr, (a1, v)) (finz.seq_between b e)) ws))) b0 e0 v0)
-      with (hash (lword_get_word <$> ws)).
-    2: {
-      rewrite /hash_lmemory_region.
-      f_equal.
-      f_equal.
-      destruct H2 as [? _]; simplify_map_eq.
-      rewrite map_filter_insert_not; cycle 1.
-      { intros w' [ ? ? ]; cbn in *; simplify_eq. }
+  Lemma wp_hash_success_same Ep pc_p pc_b pc_e pc_a pc_a' pc_v lw src wsrc :
 
-
-      Set Nested Proofs Allowed.
-  Lemma map_filter_alt':
-    ∀ {K : Type} {M : Type → Type} {H : FMap M} {H0 : ∀ A : Type, Lookup K A (M A)} {H1 : ∀ A : Type, Empty (M A)}
-      {H2 : ∀ A : Type, PartialAlter K A (M A)} {H3 : OMap M} {H4 : Merge M} {H5 : ∀ A : Type, MapFold K A (M A)}
-      {EqDecision0 : EqDecision K},
-      FinMap K M
-    → ∀ {A : Type} (P : K * A → Prop) {H7 : ∀ x : K * A, Decision (P x)}
-        (l : list (K * A)),
-        NoDup l ->
-        filter P l = map_to_list (filter P (list_to_map l)).
-    Proof.
-      intros * ? * Hnodup.
-      induction l; cbn.
-      - by rewrite map_filter_empty map_to_list_empty.
-      - apply NoDup_cons in Hnodup. destruct Hnodup as [Hal Hnodup].
-        destruct a as [a1 a2].
-        destruct (decide (P (a1,a2))); rewrite IHl; auto.
-        + rewrite map_filter_insert_True; last done; cbn.
-          admit.
-        + rewrite map_filter_insert_False; last done; cbn.
-          admit.
-    Admitted.
-    admit.
-    (* rewrite map_filter_alt'. *)
-    }
-    iFrame.
-    iDestruct (big_sepM_insert with "Hmem") as "[Ha Hmem]".
-    { apply not_elem_of_list_to_map.
-      rewrite fst_zip.
-      2: { by rewrite Hlen_ws map_length finz_seq_between_length. }
-      intro Hcontra.
-      apply elem_of_list_fmap in Hcontra.
-      destruct Hcontra as [? [? ?] ]; simplify_eq.
-    }
-    iFrame.
-    iDestruct ( big_sepM_to_big_sepL2 with "Hmem") as "Hmem".
-    { apply NoDup_fmap_2.
-      - intros a1 a2 Haeq; congruence.
-      - by apply finz_seq_between_NoDup.
-    }
-    { by rewrite Hlen_ws map_length finz_seq_between_length. }
-    iFrame.
-
-    Unshelve.
-    {
-      apply not_elem_of_list_to_map_1.
-      intro Hcontra.
-      eapply fst_elem_of_cons, elem_of_list_fmap in Hcontra.
-      destruct Hcontra as [? [? ?] ]; simplify_eq.
-    }
-  Admitted.
-
-  Lemma wp_hash_success_same Ep
-    pc_p pc_b pc_e pc_a pc_a' pc_v
-    dst p b e a v ws lw
-    :
-
-    decodeInstrWL lw = Hash dst dst →
+    decodeInstrWL lw = Hash src src →
     isCorrectLPC (LCap pc_p pc_b pc_e pc_a pc_v) →
-    readAllowed p = true →
     (pc_a + 1)%a = Some pc_a' →
 
     {{{ ▷ PC ↦ᵣ LCap pc_p pc_b pc_e pc_a pc_v
         ∗ ▷ (pc_a, pc_v) ↦ₐ lw
-        ∗ ▷ dst ↦ᵣ LCap p b e a v
-        ∗ ▷ [[ b , e ]] ↦ₐ{ v } [[ ws ]]
+        ∗ ▷ src ↦ᵣ wsrc
     }}}
       Instr Executable @ Ep
       {{{ RET NextIV;
           PC ↦ᵣ LCap pc_p pc_b pc_e pc_a' pc_v
           ∗ (pc_a, pc_v) ↦ₐ lw
-          ∗ dst ↦ᵣ LWInt (hash (lword_get_word <$> ws))
-          ∗ [[ b , e ]] ↦ₐ{ v } [[ ws ]]
+          ∗ src ↦ᵣ LWInt (hash (lword_get_word wsrc))
       }}}.
   Proof.
-  Admitted.
+    intros Hdecode HcorrectPC Hpca'.
+    iIntros (φ) "(>HPC & >Hpca & >Hsrc) Hφ".
+    iDestruct (map_of_regs_2 with "HPC Hsrc") as "[Hmap %]".
+    rewrite /region_mapsto.
+    iApply (wp_hash with "[$]"); eauto.
+    { by simplify_map_eq. }
+    { by rewrite !dom_insert; set_solver+. }
+    iNext. iIntros (lregs' retv) "(%Hspec & Hpca & Hregs)".
+    destruct Hspec; cycle 1.
+    { incrementLPC_inv; simplify_map_eq; eauto; congruence. }
+    iApply "Hφ".
+    incrementLPC_inv; simplify_map_eq; eauto.
+    rewrite (insert_commute _ PC src) // insert_insert.
+    rewrite (insert_commute _ src PC) // insert_insert.
+    iDestruct (regs_of_map_2 with "Hregs") as "(?&?)"; eauto; iFrame.
+  Qed.
 
-  Lemma wp_hash_success_overlapPC Ep
-    pc_p pc_b pc_e pc_a pc_a' pc_v
-    dst src
-    wdst p b e a v ws ws' lw
-    :
+  (* Lemma wp_hash_success_overlapPC Ep *)
+  (*   pc_p pc_b pc_e pc_a pc_a' pc_v *)
+  (*   dst src *)
+  (*   wdst p b e a v ws ws' lw *)
+  (*   : *)
 
-    decodeInstrWL lw = Hash dst src →
-    isCorrectLPC (LCap pc_p pc_b pc_e pc_a pc_v) →
-    readAllowed p = true →
-    (pc_a + 1)%a = Some pc_a' →
+  (*   decodeInstrWL lw = Hash dst src → *)
+  (*   isCorrectLPC (LCap pc_p pc_b pc_e pc_a pc_v) → *)
+  (*   readAllowed p = true → *)
+  (*   (pc_a + 1)%a = Some pc_a' → *)
 
-    {{{ ▷ PC ↦ᵣ LCap pc_p pc_b pc_e pc_a pc_v
-        ∗ ▷ dst ↦ᵣ wdst
-        ∗ ▷ src ↦ᵣ LCap p b e a v
-        ∗ ▷ [[ b , pc_a ]] ↦ₐ{ v } [[ ws ]]
-        ∗ ▷ (pc_a, pc_v) ↦ₐ lw
-        ∗ ▷ [[ pc_a' , e ]] ↦ₐ{ v } [[ ws' ]]
-    }}}
-      Instr Executable @ Ep
-      {{{ RET NextIV;
-          PC ↦ᵣ LCap pc_p pc_b pc_e pc_a' pc_v
-          ∗ dst ↦ᵣ LWInt (hash (lword_get_word <$> (ws++[lw]++ws')))
-          ∗ src ↦ᵣ LCap p b e a v
-          ∗ [[ b , pc_a ]] ↦ₐ{ v } [[ ws ]]
-          ∗ (pc_a, pc_v) ↦ₐ lw
-          ∗ [[ pc_a' , e ]] ↦ₐ{ v } [[ ws' ]]
-      }}}.
-  Proof.
-  Admitted.
+  (*   {{{ ▷ PC ↦ᵣ LCap pc_p pc_b pc_e pc_a pc_v *)
+  (*       ∗ ▷ dst ↦ᵣ wdst *)
+  (*       ∗ ▷ src ↦ᵣ LCap p b e a v *)
+  (*       ∗ ▷ [[ b , pc_a ]] ↦ₐ{ v } [[ ws ]] *)
+  (*       ∗ ▷ (pc_a, pc_v) ↦ₐ lw *)
+  (*       ∗ ▷ [[ pc_a' , e ]] ↦ₐ{ v } [[ ws' ]] *)
+  (*   }}} *)
+  (*     Instr Executable @ Ep *)
+  (*     {{{ RET NextIV; *)
+  (*         PC ↦ᵣ LCap pc_p pc_b pc_e pc_a' pc_v *)
+  (*         ∗ dst ↦ᵣ LWInt (hash (lword_get_word <$> (ws++[lw]++ws'))) *)
+  (*         ∗ src ↦ᵣ LCap p b e a v *)
+  (*         ∗ [[ b , pc_a ]] ↦ₐ{ v } [[ ws ]] *)
+  (*         ∗ (pc_a, pc_v) ↦ₐ lw *)
+  (*         ∗ [[ pc_a' , e ]] ↦ₐ{ v } [[ ws' ]] *)
+  (*     }}}. *)
+  (* Proof. *)
+  (* Admitted. *)
 
 End cap_lang_rules.
